RocqOfRust/revm/revm_interpreter/instructions/links/control/return_inner.v
@@ -41,13 +41,40 @@ Instance run_return_inner
     unit.
 Proof.
   constructor.
-  destruct run_InterpreterTypes_for_WIRE.
+  destruct run_InterpreterTypes_for_WIRE eqn:?.
   destruct run_StackTrait_for_Stack.
   destruct run_LoopControl_for_Control.
+  pose proof run_MemoryTrait_for_Memory as run_MemoryTrait_for_Memory_copy.
   destruct run_MemoryTrait_for_Memory.
   destruct run_Deref_for_Synthetic.
   destruct Impl_Default_for_Bytes.run.
   destruct (Impl_Into_for_From_T.run Impl_From_Vec_u8_for_Bytes.run).
   run_symbolic.
+  all: match goal with
+  | |- Run.Trait
+      (interpreter.interpreter.Impl_revm_interpreter_interpreter_Interpreter_IW.halt _)
+      _ _ _ _ =>
+      eapply Impl_Interpreter.run_halt
+  | |- Run.Trait
+      (interpreter.interpreter.Impl_revm_interpreter_interpreter_Interpreter_IW.halt_underflow _)
+      _ _ _ _ =>
+      eapply Impl_Interpreter.run_halt_underflow
+  | |- Run.Trait
+      (interpreter.interpreter.Impl_revm_interpreter_interpreter_Interpreter_IW.halt_overflow _)
+      _ _ _ _ =>
+      eapply Impl_Interpreter.run_halt_overflow
+  | |- Run.Trait
+      (interpreter.interpreter.Impl_revm_interpreter_interpreter_Interpreter_IW.halt_memory_oog _)
+      _ _ _ _ =>
+      eapply Impl_Interpreter.run_halt_memory_oog
+  | |- Run.Trait
+      shared_memory.interpreter.shared_memory.resize_memory
+      _ _ _ _ =>
+      eapply (@shared_memory.run_resize_memory _ _ _ _ _ _ run_MemoryTrait_for_Memory_copy)
+  | |- Run.Trait
+      interpreter_action.interpreter_action.Impl_revm_interpreter_interpreter_action_InterpreterAction.new_return
+      _ _ _ _ =>
+      typeclasses eauto
+  end.
 Defined.
 Global Opaque run_return_inner.
