RocqOfRust/revm/revm_interpreter/instructions/simulate/control/pc.v
@@ -6,6 +6,7 @@ Require Import revm.revm_interpreter.gas.simulate.constants.
 Require Import revm.revm_interpreter.instructions.links.control.pc.
 Require Import revm.revm_interpreter.instructions.simulate.macros.
 Require Import revm.revm_interpreter.links.gas.
+Require Import revm.revm_interpreter.links.instruction_context.
 Require Import revm.revm_interpreter.links.instruction_result.
 Require Import revm.revm_interpreter.links.interpreter.
 Require Import revm.revm_interpreter.links.interpreter_action.
@@ -24,13 +25,12 @@ Definition pc
     {IInterpreterTypes : InterpreterTypes.C WIRE_types}
     (interpreter : Interpreter.t WIRE WIRE_types) :
     Interpreter.t WIRE WIRE_types :=
-  gas_macro interpreter constants.BASE id (fun interpreter =>
   let pc :=
     IInterpreterTypes.(InterpreterTypes.Jumps_for_Bytecode).(Jumps.pc)
       interpreter.(Interpreter.bytecode) in
   let value : aliases.U256.t := {| Uint.value := i[pc -i 1] |} in
   push_macro interpreter value id id
-  ).
+  .
 
 Lemma pc_eq
     {WIRE H : Set} `{Link WIRE} `{Link H}
@@ -43,9 +43,13 @@ Lemma pc_eq
     (_host : H) :
   let ref_interpreter := make_ref 0 in
   let ref_host := make_ref (A := H) 1 in
+  let context := {|
+    instruction_context.InstructionContext.interpreter := ref_interpreter;
+    instruction_context.InstructionContext.host := ref_host;
+  |} in
   {{
     SimulateM.eval_f
-      (run_pc run_InterpreterTypes_for_WIRE ref_interpreter ref_host)
+      (run_pc run_InterpreterTypes_for_WIRE context)
       ([interpreter; _host]%stack) 🌲
     (
       Output.Success tt,
@@ -55,7 +59,6 @@ Lemma pc_eq
 Proof.
   intros.
   with_strategy transparent [run_pc] unfold pc, run_pc; cbn.
-  gas_macro_eq idtac.
   s. {
     apply InterpreterTypesEq.
   }
